feat: support udiv in bv_decide (#5628)
Co-authored-by: Siddharth <siddu.druid@gmail.com>

src/Std/Tactic/BVDecide/Bitblast/BVExpr/Basic.lean
@@ -65,6 +65,10 @@ inductive BVBinOp where
   Multiplication.
   -/
   | mul
+  /--
+  Unsigned division.
+  -/
+  | udiv
 
 namespace BVBinOp
 
@@ -74,6 +78,7 @@ def toString : BVBinOp → String
   | xor => "^"
   | add => "+"
   | mul => "*"
+  | udiv => "/ᵤ"
 
 instance : ToString BVBinOp := ⟨toString⟩
 
@@ -86,12 +91,14 @@ def eval : BVBinOp → (BitVec w → BitVec w → BitVec w)
   | xor => (· ^^^ ·)
   | add => (· + ·)
   | mul => (· * ·)
+  | udiv => (· / ·)
 
 @[simp] theorem eval_and : eval .and = ((· &&& ·) : BitVec w → BitVec w → BitVec w) := by rfl
 @[simp] theorem eval_or : eval .or = ((· ||| ·) : BitVec w → BitVec w → BitVec w) := by rfl
 @[simp] theorem eval_xor : eval .xor = ((· ^^^ ·) : BitVec w → BitVec w → BitVec w) := by rfl
 @[simp] theorem eval_add : eval .add = ((· + ·) : BitVec w → BitVec w → BitVec w) := by rfl
 @[simp] theorem eval_mul : eval .mul = ((· * ·) : BitVec w → BitVec w → BitVec w) := by rfl
+@[simp] theorem eval_udiv : eval .udiv = ((· / ·) : BitVec w → BitVec w → BitVec w) := by rfl
 
 end BVBinOp
 
