src/Std/Tactic/BVDecide/Bitblast/BVExpr/Circuit/Impl/Operations.lean
@@ -19,6 +19,7 @@ import Std.Tactic.BVDecide.Bitblast.BVExpr.Circuit.Impl.Operations.ShiftRight
 import Std.Tactic.BVDecide.Bitblast.BVExpr.Circuit.Impl.Operations.SignExtend
 import Std.Tactic.BVDecide.Bitblast.BVExpr.Circuit.Impl.Operations.Ult
 import Std.Tactic.BVDecide.Bitblast.BVExpr.Circuit.Impl.Operations.ZeroExtend
+import Std.Tactic.BVDecide.Bitblast.BVExpr.Circuit.Impl.Operations.Udiv
 
 /-!
 This directory contains the implementations of bitblasters for all basic operations on `BVExpr`
